In middle of proving equivalence of translating antecedents

ST/Translation.v
@@ -8,6 +8,7 @@ Require Export RelationClasses.
 Require Export Morphisms.
 Import ListNotations.
 Open Scope string_scope.
+From ST Require Import EVarsScratchwork.
 From ST Require Export ST.SoftType.
 From ST Require Import Logic VariadicQuantifiers.
 Import VectorNotations.
@@ -80,6 +81,10 @@ end.
 
 (* Consider: shift everything by 1, and have [BVar 0] reserved for future
 use in translating judgements. *)
+(* Convention: 
+translate (ad::tl, R) = And (left_fold And (map translate tl) (translate ad))
+                            (translate R).
+*)
 Global Instance TranslatableSoftType : Translatable SoftType := {
   translate (T : SoftType) :=
   match T with
@@ -103,13 +108,17 @@ in (translate st)
       (translate (Mode 3 "Manifold" [(Var (FVar "x")); (constant "c"); (Var (BVar 3))])).
 Proof. unfold constant; simpl; auto. Qed.
 
+(* The [capture_free_subst] usage here requires shifting, then unshifting,
+the bound variables. Otherwise, we end up with accidentally capturing the
+wrong variables later on. 
 
-(* The [capture_free_subst] usage here causes problems later on, so I need to think
-very carefully about what to do here... *)
+We are assuming the translation of any [SoftType] is a conjunction of
+predicates whose first argument corresponds to a [Term]. This is the whole
+design of soft type systems, after all. *)
 Global Instance TranslatableJudgementType : Translatable JudgementType := {
   translate (J : JudgementType) := 
   match J with
-  | Esti tm Tp => capture_free_subst 0 tm (translate Tp) (* XXX this needs to be carefully thought through... *)
+  | Esti tm Tp => unshift (capture_free_subst 0 (shift tm) (translate Tp))
   | Subtype T1 T2 => match (translate T1), (translate T2) with
                      | A1, A2 => Forall (Implies A1 A2)
                      end
@@ -146,39 +155,289 @@ _         __   _                         _                 __       _ _
                       |___/
 
 *)
-(* TODO: double check this works with nameless local contexts. *)
-Fixpoint translate_antecedent (lc : LocalContext) (j : JudgementType) : Formula :=
+Fixpoint naive_curried_translate_antecedent (lc : LocalContext) (j : JudgementType) : Formula :=
 match lc with
 | List.nil => translate j
 | List.cons T tl => if null tl then Forall (Implies (translate T) (translate j))
-                    else Forall (Implies (translate T) (translate_antecedent tl j))
+                    else Forall (Implies (translate T) (naive_curried_translate_antecedent tl j))
 end.
 
-Compute (translate_antecedent [(mk_mode "T1" []%vector) ; (mk_mode "T2" [(Var (BVar 0))]%vector)]%list
-(Esti (Fun "f" [(Var (BVar 1));(Var (BVar 0))]) (mk_mode "T3" [(Var (BVar 0));(Var (BVar 1))]%vector))).
+Definition curried_translate_antecedent (lc : LocalContext) (j : JudgementType) : Formula :=
+match lc with
+| List.nil => translate j
+| List.cons T tl => List.fold_left (fun a => fun b => Forall (Implies b a))
+                     (List.rev (map translate lc)) (translate j)
+end.
+
+Theorem curried_translate_equiv : forall (lc : LocalContext) (j : JudgementType),
+  curried_translate_antecedent lc j = naive_curried_translate_antecedent lc j.
+Proof.
+  intros.
+  induction lc.
+  - simpl; auto.
+  - destruct lc.
+  + simpl; auto.
+  + assert(naive_curried_translate_antecedent (a :: s ::lc)%list j
+          = Forall (Implies (translate a) (naive_curried_translate_antecedent (s ::lc)%list j))). {
+      simpl; auto.
+    }
+    rewrite H. rewrite <- IHlc. 
+    assert (curried_translate_antecedent (a :: s :: lc)%list j
+            = List.fold_left (fun a => fun b => Forall (Implies b a))
+                     (List.rev (map translate (a :: s :: lc)%list)) (translate j)). {
+      unfold curried_translate_antecedent; reflexivity.
+
+    }
+    assert(List.fold_left (fun a => fun b => Forall (Implies b a))
+    (List.rev (map translate (a::(s :: lc))%list)) (translate j)
+    = List.fold_left (fun a => fun b => Forall (Implies b a))
+    (List.rev (((translate a) :: ((translate s) :: (map translate lc)))%list)) (translate j)). {
+      simpl; auto.
+    }
+    assert (List.fold_left (fun a => fun b => Forall (Implies b a))
+    (List.rev (((translate a) :: ((translate s) :: (map translate lc)))%list)) (translate j) = 
+    List.fold_left (fun a => fun b => Forall (Implies b a))
+    ((List.rev ((translate s) :: (map translate lc)) ++ [translate a])%list) (translate j)). {
+      simpl; auto.
+    }
+    assert (List.fold_left (fun a => fun b => Forall (Implies b a))
+    (List.rev ((translate s) :: (map translate lc)) ++ [translate a])%list (translate j)
+    = List.fold_left (fun a => fun b => Forall (Implies b a))
+    (List.rev (([translate a] ++ ((translate s) :: (map translate lc)))%list)) (translate j)). {
+      simpl; auto.
+    }
+    assert (fold_left (fun a b : Formula => Forall (Implies b a))
+       (rev ([translate a] ++ translate s :: map translate lc))
+       (translate j)
+    = fold_left (fun a b : Formula => Forall (Implies b a))
+       ((rev (translate s :: map translate lc)) ++ [translate a])
+       (translate j)). {
+      simpl; auto.
+    }
+    assert (fold_left (fun a b : Formula => Forall (Implies b a))
+       ((rev (translate s :: map translate lc)) ++ [translate a])
+       (translate j)
+    = fold_left (fun a b : Formula => Forall (Implies b a))
+      [translate a]%list (fold_left (fun a b : Formula => Forall (Implies b a))
+                          (rev (translate s :: map translate lc))
+                          (translate j))). {
+      apply (List.fold_left_app (fun a b : Formula => Forall (Implies b a))). 
+    }
+    rewrite H5 in H4. rewrite H4 in H3.
+    rewrite H3 in H2. rewrite H2 in H1. rewrite H1 in H0. assumption.
+Qed.
+
+Example curried_translate_antecedent_ex2 : 
+(curried_translate_antecedent [(mk_mode "T1" []%vector) ; (mk_mode "T2" [(Var (BVar 0))]%vector)]%list
+(Esti (Fun "f" [(Var (BVar 1));(Var (BVar 0))]) (mk_mode "T3" [(Var (BVar 0));(Var (BVar 1))]%vector)))
+(* Expected: *)
+= Forall (Implies (Atom (P 1 "Mode_T1" [Var (BVar 0)]))
+                  (Forall (Implies (Atom (P 2 "Mode_T2" [Var (BVar 0); Var (BVar 1)]))
+                                   (Atom (P 3 "Mode_T3" [Fun "f" [Var (BVar 1); Var (BVar 0)]; Var (BVar 0); Var (BVar 1)]))))).
+Proof. simpl; auto. Qed.
+
 
 (* Translate [[(x : T1, y : T2(x))](f(x,y) : T3(y,x))]. *)
 (* Expected: Forall x (Forall y (|T1|(x) /\ |T2|(y,x) -> |T3|(f(x,y), y, x)))
+             Forall x, |T1|(x) -> Forall y |T2|(y,x) -> |T3|(f(x,y), y, x)
 Or namelessly: Forall (Forall (|T1|(1) /\ |T2|(0,1) -> |T3|(f(1,0), 0,1))). *)
-(* XXX Currently broken, so I goofed somewhere :( *)
-Example translate_antecedent_ex1 : 
-(translate_antecedent [(mk_mode "T1" []%vector) ; (mk_mode "T2" [(Var (BVar 0))]%vector)]%list
+Example curried_translate_antecedent_ex1 : 
+(curried_translate_antecedent [(mk_mode "T1" []%vector) ; (mk_mode "T2" [(Var (BVar 0))]%vector)]%list
 (Esti (Fun "f" [(Var (BVar 1));(Var (BVar 0))]) (mk_mode "T3" [(Var (BVar 0));(Var (BVar 1))]%vector)))
 (* Expected: *)
-= Forall (Implies (Atom (P 1 "Mode_T1" [Var (BVar )]))
-                  (Forall (Implies (Atom (P 2 "Mode_T2" [Var (BVar 1); Var (BVar 0)])))
-                                   (Atom (P 3 "Mode_T3" [Fun "f" [Var (BVar 1); Var (BVar 0)]; Var (BVar 0); Var (BVar 1)])))).
-(* Actual:
-= Forall (Implies (Atom (P 1 "Mode_T1" [Var (BVar )]))
-                  (Forall (Implies (Atom (P 2 "Mode_T2" [Var (BVar 0); Var (BVar 1)])))
-                                   (Atom (P 3 "Mode_T3" [Fun "f" [Var (BVar 1); Var (BVar 0)]; Var (BVar 1); Var (BVar 2)])))). *)
+= Forall (Implies (Atom (P 1 "Mode_T1" [Var (BVar 0)]))
+                  (Forall (Implies (Atom (P 2 "Mode_T2" [Var (BVar 0); Var (BVar 1)]))
+                                   (Atom (P 3 "Mode_T3" [Fun "f" [Var (BVar 1); Var (BVar 0)]; Var (BVar 0); Var (BVar 1)]))))).
+Proof. simpl; auto. Qed.
 
-(* Or possibly...
-= Forall (Forall (Implies (And (Atom (P 1 "Mode_T1" [Var (BVar 1)]))
-                               (Atom (P 2 "Mode_T2" [Var (BVar 1); Var (BVar 0)])))
-                          (Atom (P 3 "Mode_T3" [Fun "f" [Var (BVar 1); Var (BVar 0)]; Var (BVar 0); Var (BVar 1)])))). *)
+Example curried_translate_antecedent_ex23 :
+let field_mode := mk_mode "Field" []%vector
+in let vector_space_mode := mk_mode "VectorSpace" [(Var (BVar 0))]%vector
+in let lie_algebra_mode := mk_mode "LieAlgebra" [(Var (BVar 0)); (Var (BVar 1))]%vector
+in let affine_lie_algebra_mode := mk_mode "AffineLieAlgebra" [(Var (BVar 2)); (Var (BVar 0)); (Var (BVar 1))]%vector
+in (curried_translate_antecedent
+    [field_mode ; vector_space_mode ; lie_algebra_mode ]%list
+    (Esti (Fun "f" [(Var (BVar 1));(Var (BVar 0))]) affine_lie_algebra_mode))
+= Forall (Implies (translate field_mode)
+                  (Forall 
+                    (Implies (translate vector_space_mode)
+                             (Forall
+                              (Implies (translate lie_algebra_mode)
+                                       (translate (Esti (Fun "f" [(Var (BVar 1));(Var (BVar 0))]) affine_lie_algebra_mode))))))).
+Proof. simpl; auto. Qed.
+
+(** The uncurried version is preferable for proving properties
+of the translation process. For example, we will take advantage of the
+fact that a large class of well-typed derivations translate to a trivial
+derivation of the form [Every n (Implies p Verum)]. It is a nightmare
+to prove this using the curried version. *)
+Fixpoint right_and (a b : Formula) : Formula :=
+match a with
+| And a1 a2 => And a1 (right_and a2 b)
+| _ => And a b
+end.
+
+Require Import Coq.Bool.Bool.
+
+Lemma right_and_def : forall (a b : Formula),
+  false = is_and a -> right_and a b = And a b.
+Proof.
+  intros; simpl; auto. unfold right_and.
+  destruct a.
+  simpl; auto. simpl; auto.
+  contradict H; simpl; auto.
+  simpl; auto. simpl; auto. simpl; auto.
+Qed.
+
+Definition right_conjoin_many (h : Formula) (tl : list Formula) : Formula :=
+  List.fold_left (fun current => fun next => (right_and (shift current) next))
+    tl h.
+
+(* List.fold_left conventions are so weird, I better have a smoke check. *)
+Example right_conjoin_many_ex1 :
+  (let A := Atom (P 1 "A" [(Var (BVar 0))])
+in let B := Atom (P 2 "B" [(Var (BVar 0));(Var (BVar 1))])
+in let C := Atom (P 3 "C" [(Var (BVar 0));(Var (BVar 1));(Var (BVar 2))])
+in let D := Atom (P 3 "D" [(Var (BVar 0));(Var (BVar 1));(Var (BVar 2))])
+in right_conjoin_many A [B;C;D]%list)
+= And (Atom (P 1 "A" [Var (BVar 3)]))
+      (And (Atom (P 2 "B" [Var (BVar 2); Var (BVar 3)]))
+           (And (Atom (P 3 "C" [Var (BVar 1); Var (BVar 2); Var (BVar 3)]))
+                (Atom (P 3 "D" [Var (BVar 0); Var (BVar 1); Var (BVar 2)])))).
+Proof. simpl; auto. Qed.
+
+Lemma right_conjoin_many_nil : forall (h t : Formula) (tl : list Formula),
+  right_conjoin_many h []%list = h.
+Proof. intro; simpl; auto.  Qed.
+
+Theorem right_conjoin_many_step : forall (fm h : Formula) (l : list Formula),
+  right_conjoin_many fm (h::l)%list
+  = right_conjoin_many (right_and (shift fm) h) l.
+Proof.
+  intros.
+  simpl; auto.
+Qed.
+
+Definition uncurried_translate_antecedent (lc : LocalContext) (j : JudgementType) : Formula :=
+match lc with
+| List.nil => translate j
+| (h::tl)%list => Every (length lc) (Implies (right_conjoin_many (translate h) (List.map translate tl))
+                                             (translate j))
+end.
+
+Example uncurried_translate_antecedent_ex1 : 
+(uncurried_translate_antecedent [(mk_mode "T1" []%vector) ; (mk_mode "T2" [(Var (BVar 0))]%vector)]%list
+(Esti (Fun "f" [(Var (BVar 1));(Var (BVar 0))]) (mk_mode "T3" [(Var (BVar 0));(Var (BVar 1))]%vector)))
+= Every 2 (Implies (And (Atom (P 1 "Mode_T1" [Var (BVar 1)]))
+                        (Atom (P 2 "Mode_T2" [Var (BVar 0); Var (BVar 1)])))
+                   (Atom (P 3 "Mode_T3" [Fun "f" [Var (BVar 1); Var (BVar 0)]; Var (BVar 0); Var (BVar 1)]))).
+Proof. simpl; auto. Qed.
+
+Example uncurried_translate_antecedent_ex2 :
+let field_mode := mk_mode "Field" []%vector
+in let vector_space_mode := mk_mode "VectorSpace" [(Var (BVar 0))]%vector
+in let lie_algebra_mode := mk_mode "LieAlgebra" [(Var (BVar 0)); (Var (BVar 1))]%vector
+in let affine_lie_algebra_mode := mk_mode "AffineLieAlgebra" [(Var (BVar 2)); (Var (BVar 0)); (Var (BVar 1))]%vector
+in (uncurried_translate_antecedent
+    [field_mode ; vector_space_mode ; lie_algebra_mode ]%list
+    (Esti (Fun "f" [(Var (BVar 1));(Var (BVar 0))]) affine_lie_algebra_mode))
+= Every 3 (Implies (And (lift 0 2 (translate field_mode))
+                        (And (lift 0 1 (translate vector_space_mode))
+                             (translate lie_algebra_mode)))
+                   (translate (Esti (Fun "f" [(Var (BVar 1));(Var (BVar 0))]) affine_lie_algebra_mode))).
+Proof. simpl; auto. Qed.
+
+Lemma uncurried_translate_antecedent_structure :
+  forall (lc : LocalContext) (j : JudgementType),
+  lc <> []%list ->
+  exists (A : Formula), 
+  uncurried_translate_antecedent lc j
+  = Every (length lc)
+          (Implies A (translate j)).
+Proof.
+  intros. induction lc.
+  - contradict H. reflexivity.
+  - destruct lc.
+  + set (A := (right_conjoin_many (translate a) (List.map translate []%list))).
+    exists A. simpl; auto.
+  + intros. set (A := (right_conjoin_many (translate a) (List.map translate (s::lc)%list))).
+    exists A. simpl; auto.
+Qed.
+
+Lemma uncurried_translate_antecedent_ind :
+forall (a h : SoftType) (tl : LocalContext) (j : JudgementType),
+uncurried_translate_antecedent (a :: h :: tl)%list j
+= Every (length (a :: h :: tl)%list) 
+  (Implies (right_conjoin_many (right_and (shift (translate a)) (translate h)) (List.map translate tl))
+           (translate j)).
+Proof.
+  intros. simpl; auto.
+Qed.
+
+Lemma uncurried_translate_antecedent_implies_curried {Γ} :
+  forall (lc : LocalContext) (j : JudgementType),
+  uncurried_translate_antecedent lc j :: Γ
+  ⊢ curried_translate_antecedent lc j.
+Proof.  intros. 
+induction lc.
+  - assert (uncurried_translate_antecedent []%list j = translate j). { simpl; auto. }
+    rewrite H.
+    assert (curried_translate_antecedent []%list j = translate j). { simpl; auto. }
+    rewrite H0. apply ND_assume. prove_In.
+  - unfold curried_translate_antecedent.
+    unfold uncurried_translate_antecedent.
+    assert (fold_left (fun a0 b : Formula => Forall (Implies b a0))
+                      (rev (map translate (a :: lc)))
+                      (translate j)
+            = fold_left (fun a0 b : Formula => Forall (Implies b a0))
+                        [(translate a)]
+                        (fold_left (fun a0 b : Formula => Forall (Implies b a0))
+                                   (rev (map translate lc))
+                                   (translate j))). {
+      assert (fold_left (fun a0 b : Formula => Forall (Implies b a0))
+                        (rev (map translate (a :: lc)))
+                        (translate j)
+              = fold_left (fun a0 b : Formula => Forall (Implies b a0))
+                          ((rev (map translate lc)) ++ [(translate a)])
+                          (translate j)). {
+        simpl; auto.
+      } rewrite H. apply fold_left_app.
+    } rewrite H. destruct lc.
+    + assert ((map translate []) = []%list). { simpl; auto. }
+      unfold right_conjoin_many. unfold map. unfold rev.
+      assert ((fold_left
+       (fun a0 b : Formula =>
+        Forall (Implies b a0)) [] 
+       (translate j)) = translate j). { simpl; auto. }
+      rewrite H1. unfold fold_left. unfold length; unfold Every.
+      apply ND_assume; prove_In.
+    + assert (fold_left (fun a0 b : Formula => Forall (Implies b a0)) [translate a]
+              (fold_left (fun a0 b : Formula => Forall (Implies b a0))
+                          (rev (map translate (s :: lc))) (translate j)) 
+            = Forall (Implies (translate a)
+                             (List.fold_left (fun a0 b : Formula => Forall (Implies b a0))
+                                             (rev (map translate (s :: lc)))  (translate j)))). {
+        simpl; auto.
+      } rewrite H0.
 Admitted.
 
+Lemma curried_translate_antecedent_implies_uncurried {Γ} :
+  forall (lc : LocalContext) (j : JudgementType),
+  curried_translate_antecedent lc j :: Γ
+  ⊢ uncurried_translate_antecedent lc j.
+Admitted.
+
+Theorem translate_antecedent_equiv {Γ} :
+  forall (lc : LocalContext) (j : JudgementType),
+  Γ ⊢ Iff (uncurried_translate_antecedent lc j)
+          (curried_translate_antecedent lc j).
+Proof.
+  intros. apply ND_Iff_intro.
+  - apply uncurried_translate_antecedent_implies_curried.
+  - apply curried_translate_antecedent_implies_uncurried.
+Qed.
+
+Definition translate_antecedent := uncurried_translate_antecedent.
 
 Definition translate_definition (defn : LocalContext*JudgementType) : Formula :=
 match defn with
